tests/DataDependent.bpl
@@ -45,13 +45,25 @@ procedure Split#anon$2#2()
   assume i < 0;
   assume true;
 }
+procedure Net#init#3()
+  modifies C, R, M, St;
+{
+  assume C[Net#a] == 0;
+  assume R[Net#a] == 0;
+  assume C[Net#b] == 0;
+  assume R[Net#b] == 0;
+  assume C[Net#c] == 0;
+  assume R[Net#c] == 0;
+  assume C[Net#d] == 0;
+  assume R[Net#d] == 0;
+}
 const unique Net#rep: Actor;
 const unique Net#split: Actor;
 const unique Net#a: Chan (int);
 const unique Net#b: Chan (int);
 const unique Net#c: Chan (int);
 const unique Net#d: Chan (int);
-procedure Net#anon$3#entry#3()
+procedure Net#anon$3#entry#4()
   modifies C, R, M, St;
 {
   assume C#init[Net#a] == 2;
@@ -64,19 +76,19 @@ procedure Net#anon$3#entry#3()
   assume R[Net#d] == 0;
   assume (M[Net#a][0] < 0) && (M[Net#a][1] > 0);
   assume C#init == C;
-  assert {:msg "  Channel invariant might not hold on action entry (generated #0 )"} 0 <= R[Net#a];
-  assert {:msg "  Channel invariant might not hold on action entry (generated #1 )"} 0 <= C[Net#a];
-  assert {:msg "  Channel invariant might not hold on action entry (generated #2 )"} (R[Net#a] + C[Net#a]) == C#init[Net#a];
-  assert {:msg "  Channel invariant might not hold on action entry (generated #3 )"} 0 <= R[Net#b];
-  assert {:msg "  Channel invariant might not hold on action entry (generated #4 )"} 0 <= C[Net#b];
-  assert {:msg "  Channel invariant might not hold on action entry (generated #5 )"} 0 <= R[Net#c];
-  assert {:msg "  Channel invariant might not hold on action entry (generated #6 )"} 0 <= C[Net#c];
-  assert {:msg "  Channel invariant might not hold on action entry (generated #7 )"} R[Net#c] == 0;
-  assert {:msg "  Channel invariant might not hold on action entry (generated #8 )"} 0 <= R[Net#d];
-  assert {:msg "  Channel invariant might not hold on action entry (generated #9 )"} 0 <= C[Net#d];
-  assert {:msg "  Channel invariant might not hold on action entry (generated #10 )"} R[Net#d] == 0;
-  assert {:msg "  Channel invariant might not hold on action entry (generated #11 )"} R[Net#a] == (R[Net#b] + C[Net#b]);
-  assert {:msg "  Channel invariant might not hold on action entry (generated #12 )"} (forall idx$: int :: 
+  assert {:msg "  Channel invariant might not hold on action entry (generated #0)"} 0 <= R[Net#a];
+  assert {:msg "  Channel invariant might not hold on action entry (generated #1)"} 0 <= C[Net#a];
+  assert {:msg "  Channel invariant might not hold on action entry (generated #2)"} (R[Net#a] + C[Net#a]) == C#init[Net#a];
+  assert {:msg "  Channel invariant might not hold on action entry (generated #3)"} 0 <= R[Net#b];
+  assert {:msg "  Channel invariant might not hold on action entry (generated #4)"} 0 <= C[Net#b];
+  assert {:msg "  Channel invariant might not hold on action entry (generated #5)"} 0 <= R[Net#c];
+  assert {:msg "  Channel invariant might not hold on action entry (generated #6)"} 0 <= C[Net#c];
+  assert {:msg "  Channel invariant might not hold on action entry (generated #7)"} R[Net#c] == 0;
+  assert {:msg "  Channel invariant might not hold on action entry (generated #8)"} 0 <= R[Net#d];
+  assert {:msg "  Channel invariant might not hold on action entry (generated #9)"} 0 <= C[Net#d];
+  assert {:msg "  Channel invariant might not hold on action entry (generated #10)"} R[Net#d] == 0;
+  assert {:msg "  Channel invariant might not hold on action entry (generated #11)"} R[Net#a] == (R[Net#b] + C[Net#b]);
+  assert {:msg "  Channel invariant might not hold on action entry (generated #12)"} (forall idx$: int :: 
     (0 <= idx$) && (idx$ < (R[Net#b] + C[Net#b])) ==> (M[Net#b][idx$] == M[Net#a][idx$])
   );
   assert {:msg "  20.3: Channel invariant might not hold on action entry"} (M[Net#a][0] < 0) && (M[Net#a][1] > 0);
@@ -89,7 +101,7 @@ procedure Net#anon$3#entry#3()
     (0 <= i) && (i < R[Net#b]) && (AT#Mod(i, 2) == 1) ==> (M[Net#b][i] == M[Net#c][AT#Div(i, 2)])
   );
 }
-procedure Net#anon$3#Repeater#anon$0#4()
+procedure Net#anon$3#Repeater#anon$0#5()
   modifies C, R, M, St;
 {
   var St#next: State;
@@ -154,7 +166,7 @@ procedure Net#anon$3#Repeater#anon$0#4()
     (0 <= i) && (i < R[Net#b]) && (AT#Mod(i, 2) == 1) ==> (M[Net#b][i] == M[Net#c][AT#Div(i, 2)])
   );
 }
-procedure Net#anon$3#Split#anon$1#5()
+procedure Net#anon$3#Split#anon$1#6()
   modifies C, R, M, St;
 {
   var St#next: State;
@@ -220,7 +232,7 @@ procedure Net#anon$3#Split#anon$1#5()
     (0 <= i) && (i < R[Net#b]) && (AT#Mod(i, 2) == 1) ==> (M[Net#b][i] == M[Net#c][AT#Div(i, 2)])
   );
 }
-procedure Net#anon$3#Split#anon$2#6()
+procedure Net#anon$3#Split#anon$2#7()
   modifies C, R, M, St;
 {
   var St#next: State;
@@ -286,7 +298,7 @@ procedure Net#anon$3#Split#anon$2#6()
     (0 <= i) && (i < R[Net#b]) && (AT#Mod(i, 2) == 1) ==> (M[Net#b][i] == M[Net#c][AT#Div(i, 2)])
   );
 }
-procedure Net#anon$3#exit#7()
+procedure Net#anon$3#exit#8()
   modifies C, R, M, St;
 {
   assume C#init[Net#a] == 2;
